.ci/install.sh
@@ -9,7 +9,7 @@ git clone https://github.com/fstarlang/fstar-mode.el
 git clone https://dzomo:$DZOMO_TOKEN@github.com/fstarlang/fstarlang.github.io
 
 sudo apt-get install opam python3
-sudo easy_install docutils sphinx sphinx-rtd-theme
+sudo easy_install docutils sphinx==1.7.2 sphinx-rtd-theme
 
 export OPAMYES=true
 export OPAMJOBS=4
